Replace world with PCM

src/World.v
@@ -2,206 +2,47 @@ From sflib Require Import sflib.
 Require Import Coq.Classes.RelationClasses.
 From Fairness Require Import Axioms NatStructs.
 From Fairness Require Import PCM.
+From Fairness Require Import Mod.
 Require Import String.
 
 Set Implicit Arguments.
 
 
-Module World.
-  Class t : Type :=
-    mk {
-        G: Type;
-        L: Type;
-        unit: L;
-        compatible: G -> L -> Prop;
-        disjoint: L -> L -> Prop;
-        unit_compatible: forall g, compatible g unit;
-        unit_disjoint_l: forall l, disjoint unit l;
-        disjoint_comm: forall l0 l1 (DISJ: disjoint l0 l1), disjoint l1 l0;
-      }.
-
-  Section WORLD.
-    Context `{W: t}.
-
-    Lemma unit_disjoint_r: forall l, disjoint l unit.
-    Proof.
-      i. eapply disjoint_comm. eapply unit_disjoint_l.
-    Qed.
-
-    Variant update: G * L -> G * L -> Prop :=
-      | update_intro
-          (g0: G) (l0: L) (g1: G) (l1: L)
-          (UPDATE: forall
-              (COMPAT0: compatible g0 l0),
-              (<<COMPAT1: compatible g1 l1>>) /\
-                (<<CTX: forall l (COMPAT: compatible g0 l) (DISJ: disjoint l0 l),
-                    (<<COMPAT: compatible g1 l>>) /\ (<<DISJ: disjoint l1 l>>)>>))
-        :
-        update (g0, l0) (g1, l1)
-    .
-
-    Global Program Instance update_PreOrder: PreOrder update.
-    Next Obligation.
-      ii. destruct x. econs; eauto.
-    Qed.
-    Next Obligation.
-      ii. inv H; inv H0. econs. ii.
-      hexploit UPDATE; eauto. i. des.
-      hexploit UPDATE0; eauto. i. des. splits; eauto.
-      i. hexploit CTX; eauto. i. des.
-      hexploit CTX0; eauto.
-    Qed.
-
-    Lemma update_compatible g0 l0 g1 l1
-          (UPDATE: update (g0, l0) (g1, l1))
-          (COMPAT: compatible g0 l0)
-      :
-      compatible g1 l1.
-    Proof.
-      inv UPDATE. hexploit UPDATE0; eauto. i. des. auto.
-    Qed.
-  End WORLD.
-
-  Section PRODUCT.
-    Context `{W0: t}.
-    Context `{W1: t}.
-
-    Definition prod_G: Type := W0.(G) * W1.(G).
-    Definition prod_L: Type := W0.(L) * W1.(L).
-    Definition prod_unit: prod_L := (W0.(unit), W1.(unit)).
-    Definition prod_compatible: prod_G -> prod_L -> Prop :=
-      fun '(g0, g1) '(l0, l1) =>
-        (<<COMPAT0: W0.(compatible) g0 l0>>) /\ (<<COMPAT1: W1.(compatible) g1 l1>>).
-    Definition prod_disjoint: prod_L -> prod_L -> Prop :=
-      fun '(ll0, lr0) '(ll1, lr1) =>
-        (<<DISJ0: W0.(disjoint) ll0 ll1>>) /\ (<<DISJ1: W1.(disjoint) lr0 lr1>>).
-
-    Global Program Instance prod: t :=
-      @mk prod_G prod_L prod_unit prod_compatible prod_disjoint _ _ _.
-    Next Obligation.
-      destruct g; ss. split; eapply unit_compatible.
-    Qed.
-    Next Obligation.
-      destruct l as [l0 l1]. split; eapply unit_disjoint_l.
-    Qed.
-    Next Obligation.
-      destruct l0 as [ll0 lr0]. destruct l1 as [ll1 lr1].
-      ss. des. split; eapply disjoint_comm; eauto.
-    Qed.
-
-    Lemma prod_update gl0 gr0 ll0 lr0 gl1 gr1 ll1 lr1
-          (UPDATE0: @update W0 (gl0, ll0) (gl1, ll1))
-          (UPDATE1: @update W1 (gr0, lr0) (gr1, lr1))
-      :
-      update ((gl0, gr0), (ll0, lr0)) ((gl1, gr1), (ll1, lr1)).
-    Proof.
-      inv UPDATE0. inv UPDATE1. econs. i. ss. des.
-      hexploit UPDATE; eauto. hexploit UPDATE0; eauto. i. des.
-      splits; eauto. i. destruct l. des.
-      hexploit CTX; eauto. hexploit CTX0; eauto. i. des. splits; auto.
-    Qed.
-  End PRODUCT.
-End World.
-
-
 Section INVARIANT.
-  Context `{W: World.t}.
-
-  Definition local_worlds := NatMap.t World.L.
-
-  Variant worlds_wf (g: World.G) (ls: local_worlds): Prop :=
-    | worlds_wf_intro
-        (COMPATIBLE: forall tid l (GET: NatMap.find tid ls = Some l),
-            World.compatible g l)
-        (DISJOINT: forall tid0 tid1 l0 l1
-                          (NEQ: tid0 <> tid1)
-                          (GET0: NatMap.find tid0 ls = Some l0)
-                          (GET1: NatMap.find tid1 ls = Some l1),
-            World.disjoint l0 l1)
-  .
-
-  Lemma initial_worlds_wf g: worlds_wf g (NatMap.empty World.L).
-  Proof.
-    econs.
-    { i. rewrite NatMapP.F.empty_o in GET. ss. }
-    { i. rewrite NatMapP.F.empty_o in GET0. ss. }
-  Qed.
-
-  Lemma worlds_add_unit_wf g ls tid
-        (WF: worlds_wf g ls)
-    :
-    worlds_wf g (NatMap.add tid World.unit ls).
-  Proof.
-    inv WF. econs.
-    { i. rewrite NatMapP.F.add_o in GET. des_ifs.
-      { eapply World.unit_compatible. }
-      { eapply COMPATIBLE; eauto. }
-    }
-    { i. rewrite NatMapP.F.add_o in GET0. rewrite NatMapP.F.add_o in GET1. des_ifs.
-      { eapply World.unit_disjoint_r. }
-      { eapply World.unit_disjoint_l. }
-      { eapply (DISJOINT tid0 tid1); eauto. }
-    }
-  Qed.
-
-  Lemma worlds_update_wf g0 ls tid l0 g1 l1
-        (UPDATE: World.update (g0, l0) (g1, l1))
-        (GET: NatMap.find tid ls = Some l0)
-        (WF: worlds_wf g0 ls)
-    :
-    worlds_wf g1 (NatMap.add tid l1 ls).
-  Proof.
-    inv WF. inv UPDATE. hexploit UPDATE0; eauto. i. des.
-    econs.
-    { i. rewrite NatMapP.F.add_o in GET0. des_ifs.
-      eapply CTX; eauto.
-    }
-    { i. rewrite NatMapP.F.add_o in GET0. rewrite NatMapP.F.add_o in GET1. des_ifs.
-      { eapply World.disjoint_comm. eapply UPDATE0; eauto. }
-      { eapply UPDATE0; eauto. }
-      { eapply (DISJOINT tid0 tid1); eauto. }
-    }
-  Qed.
-End INVARIANT.
-
-Section PCM.
   Context `{M: URA.t}.
 
-  Definition pcm_disjoint: URA.car -> URA.car -> Prop :=
-    fun r0 r1 => forall (WF0: URA.wf r0) (WF1: URA.wf r1), URA.wf (r0 ⋅ r1).
+  Definition local_resources := NatMap.t URA.car.
 
-  (* Definition pcm_disjoint: URA.car -> URA.car -> Prop := *)
-  (*   fun r0 r1 => URA.wf (r0 ⋅ r1). *)
+  Definition unwrap_opt_resource (r: option URA.car): URA.car :=
+    match r with
+    | Some r => r
+    | None => ε
+    end.
 
-  (* Definition pcm_compatible: URA.car -> URA.car -> Prop := *)
-  (*   fun g r => forall (WF: URA.wf g), URA.wf (g ⋅ r). *)
+  Definition sum_of_resources (rs: local_resources): URA.car :=
+    NatMap.fold (fun _ r s => r ⋅ s) rs ε.
 
-  Global Program Instance pcm_world: World.t :=
-    @World.mk URA.car URA.car URA.unit pcm_disjoint pcm_disjoint _ _ _.
-  Next Obligation.
-    ii. rewrite URA.unit_id. auto.
-  Qed.
-  Next Obligation.
-    ii. rewrite URA.unit_idl. auto.
-  Qed.
-  Next Obligation.
-    ii. rewrite URA.add_comm. eapply DISJ; eauto.
-  Qed.
+  Definition resources_wf (g: URA.car) (rs: local_resources): Prop :=
+    URA.wf (g ⋅ sum_of_resources rs)
+  .
 
-  Lemma updatable_update g0 r0 g1 r1
-        (COMPAT: World.compatible g0 r0)
-        (UPDATABLE: URA.updatable (g0 ⋅ r0) (g1 ⋅ r1))
-        (WF0: URA.wf g0)
-        (WF1: URA.wf r0)
+  Definition get_resource
+             (tid: thread_id.(id))
+             (rs: local_resources)
+    : (URA.car * local_resources) :=
+    match nm_pop tid rs with
+    | Some (r, rs) => (r, rs)
+    | _ => (ε, rs)
+    end.
+
+  Lemma resources_wf_get_wf g0 tid rs0 r0 rs1
+        (WF: resources_wf g0 rs0)
+        (GET: get_resource tid rs0 = (r0, rs1))
     :
-    (<<UPDATE: World.update (g0, r0) (g1, r1)>>) /\ (<<WF0: URA.wf g1>>) /\ (<<WF1: URA.wf r1>>).
+    (<<WF: URA.wf (g0 ⋅ r0 ⋅ sum_of_resources rs1)>>) /\
+      (<<UPDATE: forall g1 r1
+                        (WF: URA.wf (g0 ⋅ r0 ⋅ sum_of_resources rs1)),
+          resources_wf g1 (NatMap.add tid r1 rs1)>>).
   Proof.
-    pose proof (UPDATABLE URA.unit) as UNIT.
-    hexploit UNIT.
-    { rewrite URA.unit_id. eapply COMPAT; eauto. }
-    i. rewrite URA.unit_id in H. splits.
-    { econs. i. splits.
-      { ii. eauto. }
-      { i. split.
-  Abort.
-End PCM.
+  Admitted.
+End INVARIANT.
